@prefix : <http://rdf.cdisc.org/mms#> .
@prefix dc: <http://purl.org/dc/elements/1.1/> .
@prefix owl: <http://www.w3.org/2002/07/owl#> .
@prefix rdf: <http://www.w3.org/1999/02/22-rdf-syntax-ns#> .
@prefix xml: <http://www.w3.org/XML/1998/namespace> .
@prefix xsd: <http://www.w3.org/2001/XMLSchema#> .
@prefix rdfs: <http://www.w3.org/2000/01/rdf-schema#> .
@prefix skos: <http://www.w3.org/2004/02/skos/core#> .
@base <http://rdf.cdisc.org/mms> .

<http://rdf.cdisc.org/mms> rdf:type owl:Ontology ;
                            owl:imports <http://www.w3.org/2004/02/skos/core> ;
                            rdfs:label "CDISC Common Meta Model Schema"^^xsd:string ;
                            skos:definition "The common CDISC Meta Model Schema defines a set of generic meta-model resources that provides a common language and infrastructure to describe the CDISC operational standards."^^xsd:string ;
                            dc:creator "NCI EVS"^^xsd:string .

#################################################################
#    Annotation properties
#################################################################

###  http://rdf.cdisc.org/mms#contextLabel
:contextLabel rdf:type owl:AnnotationProperty ;
              rdfs:subPropertyOf skos:prefLabel .


###  http://rdf.cdisc.org/mms#dataElementLabel
:dataElementLabel rdf:type owl:AnnotationProperty ;
                  rdfs:subPropertyOf skos:prefLabel .


#################################################################
#    Object Properties
#################################################################

###  http://rdf.cdisc.org/mms#broader
:broader rdf:type owl:ObjectProperty ;
         rdfs:domain :DataElement ;
         rdfs:range :DataElement ;
         rdfs:isDefinedBy <http://rdf.cdisc.org/mms> ;
         rdfs:label "Broader"^^xsd:string ;
         skos:definition "Relates a data element to another data element that is more general."^^xsd:string .


###  http://rdf.cdisc.org/mms#context
:context rdf:type owl:ObjectProperty ;
         rdfs:domain :AdministeredItem ;
         rdfs:range :Context ;
         rdfs:isDefinedBy <http://rdf.cdisc.org/mms> ;
         rdfs:label "Context"^^xsd:string ;
         skos:definition "The context of an administered item."^^xsd:string .


###  http://rdf.cdisc.org/mms#dataElement
:dataElement rdf:type owl:ObjectProperty ;
             rdfs:domain :DataElementContext ;
             rdfs:range :DataElement ;
             rdfs:isDefinedBy <http://rdf.cdisc.org/mms> ;
             rdfs:label "Data Element"^^xsd:string ;
             skos:definition "The data element that a data element context refers to."^^xsd:string .


###  http://rdf.cdisc.org/mms#dataElementValueDomain
:dataElementValueDomain rdf:type owl:ObjectProperty ;
                        rdfs:domain :DataElement ;
                        rdfs:range :ValueDomain ;
                        rdfs:isDefinedBy <http://rdf.cdisc.org/mms> ;
                        rdfs:label "Data Element Value Domain"^^xsd:string ;
                        skos:definition "The value domain of a data element."^^xsd:string .


###  http://rdf.cdisc.org/mms#inValueDomain
:inValueDomain rdf:type owl:ObjectProperty ;
               rdfs:domain :PermissibleValue ;
               rdfs:range :EnumeratedValueDomain ;
               rdfs:isDefinedBy <http://rdf.cdisc.org/mms> ;
               rdfs:label "Value Domain"^^xsd:string ;
               skos:definition "The enumerated value domain to which a permissible value belongs."^^xsd:string .


###  http://rdf.cdisc.org/mms#subsetOf
:subsetOf rdf:type owl:ObjectProperty ;
          rdfs:domain :EnumeratedValueDomain ;
          rdfs:range :EnumeratedValueDomain ;
          rdfs:isDefinedBy <http://rdf.cdisc.org/mms> ;
          rdfs:label "Parent Value Domain"^^xsd:string ;
          skos:definition "Identifies the parent enumerated value domain of which this enumerated value domain is a subset of."^^xsd:string .


#################################################################
#    Data properties
#################################################################

###  http://rdf.cdisc.org/mms#contextDescription
:contextDescription rdf:type owl:DatatypeProperty ;
                    rdfs:domain :Context ;
                    rdfs:range xsd:string ;
                    rdfs:isDefinedBy <http://rdf.cdisc.org/mms> ;
                    rdfs:label "Context Description"^^xsd:string ;
                    skos:definition "The descriptive text documenting a context."^^xsd:string .


###  http://rdf.cdisc.org/mms#contextLabel
:contextLabel rdf:type owl:DatatypeProperty ;
              rdfs:domain :Context ;
              rdfs:range xsd:string .


###  http://rdf.cdisc.org/mms#contextName
:contextName rdf:type owl:DatatypeProperty ;
             rdfs:domain :Context ;
             rdfs:range xsd:string ;
             rdfs:isDefinedBy <http://rdf.cdisc.org/mms> ;
             rdfs:label "Context Name"^^xsd:string ;
             skos:definition "The name of a context that uniquely identifies it within the registry."^^xsd:string .


###  http://rdf.cdisc.org/mms#dataElementDescription
:dataElementDescription rdf:type owl:DatatypeProperty ;
                        rdfs:domain :DataElement ;
                        rdfs:range xsd:string ;
                        rdfs:isDefinedBy <http://rdf.cdisc.org/mms> ;
                        rdfs:label "Data Element Description"^^xsd:string ;
                        skos:definition "The descriptive text documenting a data element."^^xsd:string .


###  http://rdf.cdisc.org/mms#dataElementLabel
:dataElementLabel rdf:type owl:DatatypeProperty ;
                  rdfs:domain :DataElement ;
                  rdfs:range xsd:string .


###  http://rdf.cdisc.org/mms#dataElementName
:dataElementName rdf:type owl:DatatypeProperty ;
                 rdfs:domain :DataElement ;
                 rdfs:range xsd:string ;
                 rdfs:isDefinedBy <http://rdf.cdisc.org/mms> ;
                 rdfs:label "Data Element Name"^^xsd:string ;
                 skos:definition "The name of a data element that uniquely identifies it within a context."^^xsd:string ;
                 skos:note "A distinction must be made between the unique URI identifying a data element as a resource within the ontology and the name of a data element used to identify it within a context."^^xsd:string .


###  http://rdf.cdisc.org/mms#dataElementType
:dataElementType rdf:type owl:DatatypeProperty ;
                 rdfs:domain :DataElement ;
                 rdfs:range xsd:string ;
                 rdfs:isDefinedBy <http://rdf.cdisc.org/mms> ;
                 rdfs:label "Data Element Type"^^xsd:string ;
                 skos:definition "The type of a data element, i.e. the values it can range over. The actual value space may be further restricted by the specification of a value domain."^^xsd:string .


###  http://rdf.cdisc.org/mms#identifier
:identifier rdf:type owl:DatatypeProperty ;
            rdfs:domain :AdministeredItem ;
            rdfs:range xsd:string ;
            rdfs:isDefinedBy <http://rdf.cdisc.org/mms> ;
            rdfs:label "Identifier"^^xsd:string ;
            skos:definition "The identifier of an administered item."^^xsd:string .


###  http://rdf.cdisc.org/mms#ordinal
:ordinal rdf:type owl:DatatypeProperty ;
         rdfs:domain :AdministeredItem ;
         rdfs:range xsd:positiveInteger ;
         rdfs:isDefinedBy <http://rdf.cdisc.org/mms> ;
         rdfs:label "Ordinal"^^xsd:string ;
         skos:definition "The ordinal of an administered item within a list of items."^^xsd:string .


#################################################################
#    Classes
#################################################################

###  http://rdf.cdisc.org/mms#AdministeredItem
:AdministeredItem rdf:type owl:Class ;
                  rdfs:subClassOf owl:Thing ;
                  rdfs:isDefinedBy <http://rdf.cdisc.org/mms> ;
                  rdfs:label "Administered Item"^^xsd:string ;
                  skos:definition "Any resource for which administrative information is recorded in an administration record."^^xsd:string .


###  http://rdf.cdisc.org/mms#Classifier
:Classifier rdf:type owl:Class ;
            rdfs:subClassOf :AdministeredItem ;
            rdfs:isDefinedBy <http://rdf.cdisc.org/mms> ;
            rdfs:label "Classifier"^^xsd:string ;
            skos:definition "A classifier defines a characteristic that can be used to organize a set of administered items into a discrete family of subsets."^^xsd:string ;
            skos:example "SDTM classifies variables to be either required, or expected, or permissible."^^xsd:string .


###  http://rdf.cdisc.org/mms#Column
:Column rdf:type owl:Class ;
        rdfs:subClassOf :DataElementContext ;
        rdfs:isDefinedBy <http://rdf.cdisc.org/mms> ;
        rdfs:label "Column"^^xsd:string ;
        skos:definition "A column is a data element in the context of a dataset and may add context dependent properties such as the ordinal number within the dataset."^^xsd:string .


###  http://rdf.cdisc.org/mms#Context
:Context rdf:type owl:Class ;
         rdfs:subClassOf :AdministeredItem ;
         rdfs:isDefinedBy <http://rdf.cdisc.org/mms> ;
         rdfs:label "Context"^^xsd:string ;
         skos:definition "Each administered item is named and defined within one or more contexts. A context defines the scope within which the subject data has meaning. A context may be a business domain, an information subject area, an information system, a database, file, data model, standard document, or any other environment determined by the owner of the registry. Each context is itself managed as an administered item within the registry and is given a name and a definition."^^xsd:string .


###  http://rdf.cdisc.org/mms#DataCollectionField
:DataCollectionField rdf:type owl:Class ;
                     rdfs:subClassOf :DataElementContext ;
                     rdfs:isDefinedBy <http://rdf.cdisc.org/mms> ;
                     rdfs:label "Data Collection Field"^^xsd:string ;
                     skos:definition "A data collection field is a data element in the context of a data collection form and may add context dependent properties such as optional or required."^^xsd:string .


###  http://rdf.cdisc.org/mms#DataCollectionForm
:DataCollectionForm rdf:type owl:Class ;
                    rdfs:subClassOf :Context ;
                    rdfs:isDefinedBy <http://rdf.cdisc.org/mms> ;
                    rdfs:label "Data Collection Form"^^xsd:string ;
                    skos:definition "Context to group a set of data collection fields."^^xsd:string .


###  http://rdf.cdisc.org/mms#DataElement
:DataElement rdf:type owl:Class ;
             rdfs:subClassOf :AdministeredItem ;
             rdfs:isDefinedBy <http://rdf.cdisc.org/mms> ;
             rdfs:label "Data Element"^^xsd:string ;
             skos:definition "Unit of data that is considered in context to be indivisible."^^xsd:string .


###  http://rdf.cdisc.org/mms#DataElementContext
:DataElementContext rdf:type owl:Class ;
                    rdfs:subClassOf :DataElement ;
                    rdfs:isDefinedBy <http://rdf.cdisc.org/mms> ;
                    rdfs:label "Data Element Context"^^xsd:string ;
                    skos:definition "A data element context maps a data element to a context and describes context dependent properties of that data element."^^xsd:string .


###  http://rdf.cdisc.org/mms#Dataset
:Dataset rdf:type owl:Class ;
         rdfs:subClassOf :Context ;
         rdfs:isDefinedBy <http://rdf.cdisc.org/mms> ;
         rdfs:label "Dataset"^^xsd:string ;
         skos:definition "Context to group a set of dataset variables, e.g. SDTM IG Adverse Event domain."^^xsd:string .


###  http://rdf.cdisc.org/mms#DatasetContext
:DatasetContext rdf:type owl:Class ;
                rdfs:subClassOf :Context ;
                rdfs:isDefinedBy <http://rdf.cdisc.org/mms> ;
                rdfs:label "Dataset Context"^^xsd:string ;
                skos:definition "Context to group related data sets, e.g. Events Observation Class."^^xsd:string .


###  http://rdf.cdisc.org/mms#Domain
:Domain rdf:type owl:Class ;
        rdfs:subClassOf :Context ;
        rdfs:isDefinedBy <http://rdf.cdisc.org/mms> ;
        rdfs:label "Data Element Domain"^^xsd:string ;
        skos:definition "Context to group a set of related data elements."^^xsd:string .


###  http://rdf.cdisc.org/mms#DomainContext
:DomainContext rdf:type owl:Class ;
               rdfs:subClassOf :Context ;
               rdfs:isDefinedBy <http://rdf.cdisc.org/mms> ;
               rdfs:label "Domain Context"^^xsd:string ;
               skos:definition "Context to group related domains."^^xsd:string .


###  http://rdf.cdisc.org/mms#EnumeratedValueDomain
:EnumeratedValueDomain rdf:type owl:Class ;
                       rdfs:subClassOf :ValueDomain ;
                       rdfs:isDefinedBy <http://rdf.cdisc.org/mms> ;
                       rdfs:label "Enumerated Value Domain"^^xsd:string ;
                       skos:definition "A Value Domain that is specified by a list of all its Permissible Values."^^xsd:string .


###  http://rdf.cdisc.org/mms#Model
:Model rdf:type owl:Class ;
       rdfs:subClassOf :Context ;
       rdfs:isDefinedBy <http://rdf.cdisc.org/mms> ;
       rdfs:label "Model"^^xsd:string ;
       skos:definition "Top-level context for all model elements, e.g. SDTM 3.1.2."^^xsd:string .


###  http://rdf.cdisc.org/mms#PermissibleValue
:PermissibleValue rdf:type owl:Class ;
                  rdfs:subClassOf :AdministeredItem ;
                  rdfs:isDefinedBy <http://rdf.cdisc.org/mms> ;
                  rdfs:label "Permissible Value"^^xsd:string ;
                  skos:definition "A permissible value is a designation, binding of signs (value) to a corresponding value meaning."^^xsd:string .


###  http://rdf.cdisc.org/mms#ValueDomain
:ValueDomain rdf:type owl:Class ;
             rdfs:subClassOf :AdministeredItem ;
             rdfs:isDefinedBy <http://rdf.cdisc.org/mms> ;
             rdfs:label "Value Domain"^^xsd:string ;
             skos:definition "A value domain is a collection of permissible values. A value domain provides representation, but has no implication as to what data element concept the values are associated with, nor what the values mean."^^xsd:string .


###  http://rdf.cdisc.org/mms#VariableGrouping
:VariableGrouping rdf:type owl:Class ;
                  rdfs:subClassOf :Context ;
                  rdfs:isDefinedBy <http://rdf.cdisc.org/mms> ;
                  rdfs:label "Variable Grouping"^^xsd:string ;
                  skos:definition "Context to group a set of data elements, e.g. SDTM Timing Variables."^^xsd:string .


#################################################################
#    Annotations
#################################################################

:contextLabel skos:definition "Short descriptive label of a context."^^xsd:string ;
              rdfs:label "Context Label"^^xsd:string ;
              rdfs:isDefinedBy <http://rdf.cdisc.org/mms> .


:dataElementLabel skos:definition "Short descriptive label of a data element."^^xsd:string ;
                  rdfs:label "Data Element Label"^^xsd:string ;
                  rdfs:isDefinedBy <http://rdf.cdisc.org/mms> .


###  Generated by the OWL API (version 4.2.8.20170104-2310) https://github.com/owlcs/owlapi
